More work in connecting instances of operational semantics to their type classes.

HoareLogic/SmallStepSemantics.v
@@ -38,90 +38,54 @@ Class NormalSmallStepSemantics (P: ProgrammingLanguage) (state: Type) (SSS: Smal
 }.
 
 Definition access {P: ProgrammingLanguage} {Imp: ImperativeProgrammingLanguage P} {state: Type} {SSS: SmallStepSemantics P state} (s: state) (c: cmd) (ms: MetaState state) :=
-  
-    match ms with
-    | Terminating s0 => clos_refl_trans _ lift_step (Terminating (c, s))  (Terminating (Sskip, s0))
-    | NonTerminating => clos_refl_trans _ lift_step (Terminating (c, s)) NonTerminating \/ exists cs: nat -> cmd * state, cs 0 = (c, s) /\ forall k, step (cs k) (Terminating (cs (S k)))
-    | Error => clos_refl_trans _ lift_step (Terminating (c, s)) Error
-    end.
+  clos_refl_trans _ lift_step (Terminating (c, s)) (lift_function (pair Sskip) ms) \/
+  ms = NonTerminating /\ exists cs: nat -> cmd * state, cs 0 = (c, s) /\ forall k, step (cs k) (Terminating (cs (S k))).
 
 Class SASmallStepSemantics (P: ProgrammingLanguage) (state: Type) {J: Join state} {kiM: KripkeIntuitionisticModel state} (SSS: SmallStepSemantics P state): Type := {
   frame_property: forall (m mf m': cmd * state) n', join (snd m) (snd mf) (snd m') -> step_safe m -> step m' n' -> exists n nf, Korder (snd nf) (snd mf) /\ @lift_join _ (@prod_Join cmd state (equiv_Join cmd) J) n (Terminating nf) n' /\ step m n
 }.
 
-Inductive loop_access_fin
-          {state: Type}
-          {kiM: KripkeIntuitionisticModel state}
-          (R: state -> MetaState state -> Prop)
-          (test: state -> Prop): state -> MetaState state -> Prop :=
-| loop_access_Terminating:
-    forall s1 s2,
-      ~ test s1 ->
-      Korder s2 s1 ->
-      loop_access_fin R test s1 (Terminating s2)
-| loop_access_Error:
-    forall s1 s2,
-      test s1 ->
-      Korder s2 s1 ->
-      R s2 Error ->
-      loop_access_fin R test s1 Error
-| loop_access_fin_NonTerminating:
-    forall s1 s2,
-      test s1 ->
-      Korder s2 s1 ->
-      R s2 NonTerminating ->
-      loop_access_fin R test s1 NonTerminating
-| loop_access_step:
-    forall s1 s2 s3 s4 ms,
-      test s1 ->
-      Korder s2 s1 ->
-      R s2 (Terminating s3) ->
-      Korder s4 s3 ->
-      loop_access_fin R test s4 ms ->
-      loop_access_fin R test s1 ms.
+Module Partial.
 
-Inductive loop_access_inf
-          {state: Type}
-          {kiM: KripkeIntuitionisticModel state}
-          (R: state -> MetaState state -> Prop)
-          (test: state -> Prop): state -> Prop :=
-| loop_access_inf_NonTerminating:
-    forall (s1 s2 s3: nat -> state),
-      (forall n, test (s1 n)) ->
-      (forall n, Korder (s2 n) (s1 n)) ->
-      (forall n, R (s2 n) (Terminating (s3 n))) ->
-      (forall n, Korder (s1 (S n)) (s3 n)) ->
-      loop_access_inf R test (s1 0).
+Class ImpSmallStepSemantics (P: ProgrammingLanguage) {iP: ImperativeProgrammingLanguage P} (state: Type) {kiM: KripkeIntuitionisticModel state} (SSS: SmallStepSemantics P state): Type := {
+  eval_bool: state -> bool_expr -> Prop;
+  eval_bool_stable: forall b, Korder_stable (fun s => eval_bool s b);
+  step_Ssequence: forall c1 c2 s mcs,
+    step (Ssequence c1 c2, s) mcs ->
+    mcs = NonTerminating \/
+    (exists s', c1 = Sskip /\ Korder s' s /\ mcs = Terminating (c2, s')) \/
+    (exists mcs', step (c2, s) mcs' /\ mcs = lift_function (fun cs => (Ssequence c1 (fst cs), snd cs)) mcs');
+  step_Sifthenelse: forall b c1 c2 s mcs,
+    step (Sifthenelse b c1 c2, s) mcs ->
+    mcs = NonTerminating \/
+    (eval_bool s b /\ exists s', Korder s' s /\ mcs = Terminating (c1, s')) \/
+    (~ eval_bool s b /\ exists s', Korder s' s /\ mcs = Terminating (c2, s'));
+  step_Swhile: forall b c s mcs,
+    step (Swhile b c, s) mcs ->
+    mcs = NonTerminating \/
+    (eval_bool s b /\ exists s', Korder s' s /\ mcs = Terminating (Ssequence c (Swhile b c), s')) \/
+    (~ eval_bool s b /\ exists s', Korder s' s /\ mcs = Terminating (Sskip, s'))
+}.
 
-Inductive loop_access
-          {state: Type}
-          {kiM: KripkeIntuitionisticModel state}
-          (R: state -> MetaState state -> Prop)
-          (test: state -> Prop): state -> MetaState state -> Prop :=
-| loop_access_loop_access_fin:
-    forall s ms, loop_access_fin R test s ms ->
-      loop_access R test s ms
-| loop_access_loop_access_inf:
-    forall s, loop_access_inf R test s ->
-      loop_access R test s NonTerminating.
-(*
+End Partial.
+
+Module Total.
+
 Class ImpSmallStepSemantics (P: ProgrammingLanguage) {iP: ImperativeProgrammingLanguage P} (state: Type) {kiM: KripkeIntuitionisticModel state} (SSS: SmallStepSemantics P state): Type := {
   eval_bool: state -> bool_expr -> Prop;
   eval_bool_stable: forall b, Korder_stable (fun s => eval_bool s b);
   step_Ssequence: forall c1 c2 s mcs,
     step (Ssequence c1 c2, s) mcs ->
     (exists s', c1 = Sskip /\ Korder s' s /\ mcs = Terminating (c2, s')) \/
-    (exists mcs', step (c2, s) mcs' /\ mcs = lift_function (fun cs => (Ssequence c1 (fst cs), snd cs)) mcs')
-}.
-    exists ms' ms'',
-      access s c1 ms' /\ lift_Korder ms'' ms' /\ lift_access ms'' c2 ms;
-  access_Sifthenelse: forall b c1 c2 s ms,
-    access s (Sifthenelse b c1 c2) ms ->
-    (eval_bool s b /\ exists s', Korder s' s /\ access s' c1 ms) \/
-    (~ eval_bool s b /\ exists s', Korder s' s /\ access s' c2 ms);
-  access_Swhile: forall b c s ms,
-    access s (Swhile b c) ms ->
-    loop_access (fun s ms => access s c ms) (fun s => eval_bool s b) s ms
+    (exists mcs', step (c2, s) mcs' /\ mcs = lift_function (fun cs => (Ssequence c1 (fst cs), snd cs)) mcs');
+  step_Sifthenelse: forall b c1 c2 s mcs,
+    step (Sifthenelse b c1 c2, s) mcs ->
+    (eval_bool s b /\ exists s', Korder s' s /\ mcs = Terminating (c1, s')) \/
+    (~ eval_bool s b /\ exists s', Korder s' s /\ mcs = Terminating (c2, s'));
+  step_Swhile: forall b c s mcs,
+    step (Swhile b c, s) mcs ->
+    (eval_bool s b /\ exists s', Korder s' s /\ mcs = Terminating (Ssequence c (Swhile b c), s')) \/
+    (~ eval_bool s b /\ exists s', Korder s' s /\ mcs = Terminating (Sskip, s'))
 }.
 
-*)
+End Total.
